README.md
@@ -12,8 +12,8 @@ lake test # run all days
 .lake/build/bin/aoc2025 2    # run day 2
 ```
 
-| Day | Date   | Problem             | Solution                       |
-|-----|--------|---------------------|--------------------------------|
+| Day | Date   | Problem                                                    | Solution                       |
+|-----|--------|------------------------------------------------------------|--------------------------------|
 | 1   | Dec 1  | [Secret Entrance](https://adventofcode.com/2025/day/1)     | [Day1.lean](AoC2025/Day1.lean) |
 | 2   | Dec 2  | [Gift Shop](https://adventofcode.com/2025/day/2)           | [Day2.lean](AoC2025/Day2.lean) |
 | 3   | Dec 3  | [Lobby](https://adventofcode.com/2025/day/3)               | [Day3.lean](AoC2025/Day3.lean) |
@@ -22,7 +22,7 @@ lake test # run all days
 | 6   | Dec 6  | [Trash Compactor](https://adventofcode.com/2025/day/6)     | [Day6.lean](AoC2025/Day6.lean) |
 | 7   | Dec 7  | [Laboratories](https://adventofcode.com/2025/day/7)        | [Day7.lean](AoC2025/Day7.lean) |
 | 8   | Dec 8  | [Playground](https://adventofcode.com/2025/day/8)          | [Day8.lean](AoC2025/Day8.lean) |
-| 9   | Dec 9  | [Movie Theater](https://adventofcode.com/2025/day/9) | [Day9.lean](AoC2025/Day9.lean) |
-| 10  | Dec 10 | TBD                 | -                              |
-| 11  | Dec 11 | TBD                 | -                              |
-| 12  | Dec 12 | TBD                 | -                              |
+| 9   | Dec 9  | [Movie Theater](https://adventofcode.com/2025/day/9)       | [Day9.lean](AoC2025/Day9.lean) |
+| 10  | Dec 10 | TBD                                                        | -                              |
+| 11  | Dec 11 | TBD                                                        | -                              |
+| 12  | Dec 12 | TBD                                                        | -                              |
